worked out a way to relate expressions with a single relation that does not depend on expression type or context, but got stuck when trying to use casts...

theories/Reflection/OExpr_untyped.v
@@ -3,81 +3,41 @@ Require Import Coq.Logic.ProofIrrelevance.
 
 Import EqNotations.
 Import ListNotations.
+Import ProofIrrelevanceTheory.
 
 
 (***
- *** Ordered Expressions
+ *** Ordered Type Contexts
  ***)
-
-(* Ordered expressions to represent proper functions *)
-Inductive OExpr : Type :=
-| OVar (n:nat)
-| OEmbed {A} {RA:OTRelation A} (a:A)
-| OApp (A B:Type) {RA:OTRelation A} {RB:OTRelation B} (e1 e2 : OExpr)
-| OLam (A B:Type) {RA:OTRelation A} {RB:OTRelation B} (e: OExpr)
-.
-
-(* Weakening / lifting of ordered expression variables *)
-Fixpoint weakenOVar n k (v:nat) {struct n} : nat :=
-  match n with
-  | 0 => v + k
-  | S n' =>
-    match v with
-    | 0 => 0
-    | S v' => weakenOVar n' k v'
-    end
-  end.
-
-(* Weakening / lifting of ordered expressions *)
-Fixpoint weakenOExpr n k (e:OExpr) : OExpr :=
-  match e with
-  | OVar v => OVar (weakenOVar n k v)
-  | OEmbed a => OEmbed a
-  | OApp A B f arg => OApp A B (weakenOExpr n k f) (weakenOExpr n k arg)
-  | OLam A B f => OLam A B (weakenOExpr (S n) k f)
-  end.
-
-(* Substitution for ordered expression variables *)
-Fixpoint substOVar n lifting (s:OExpr) v : OExpr :=
-  match n with
-  | 0 =>
-    match v with
-    | 0 => weakenOExpr 0 lifting s
-    | S v' => OVar v'
-    end
-  | S n' =>
-    match v with
-    | 0 => OVar lifting
-    | S v' =>
-      substOVar n' (S lifting) s v
-    end
-  end.
-
-(* Substitution for ordered expressions *)
-Fixpoint substOExpr n (s:OExpr) (e:OExpr) : OExpr :=
-  match e with
-  | OVar v => substOVar n 0 s v
-  | OEmbed a => OEmbed a
-  | OApp A B f arg => OApp A B (substOExpr n s f) (substOExpr n s arg)
-  | OLam A B body => OLam A B (substOExpr (S n) s body)
-  end.
-
-
-(***
- *** Typing for Ordered Expressions
- ***)
-
-(* Proof that one ordered type equals another *)
-Definition eqOType A {RA:OTRelation A} B {RB:OTRelation B} : Prop :=
-  existT OTRelation A RA = existT OTRelation B RB.
-
-
 
 (* A context here is just a list of types *)
 Inductive Ctx : Type :=
 | CtxNil
 | CtxCons A `{OTRelation A} (ctx:Ctx)
 .
+
+(* Inductive type stating that every type in a Ctx is a valid OType *)
+Inductive ValidCtxInd : Ctx -> Prop :=
+| ValidCtxNil : ValidCtxInd CtxNil
+| ValidCtxCons A `{OType A} ctx : ValidCtxInd ctx -> ValidCtxInd (CtxCons A ctx)
+.
+
+(* Inversion for ValidCtxInd *)
+Lemma ValidCtxInd_inversion A `{OTRelation A} ctx
+      (valid:ValidCtxInd (CtxCons A ctx)) : OType A /\ ValidCtxInd ctx.
+  inversion valid.
+  dependent rewrite <- H1.
+  split; assumption.
+Qed.
+
+(* Typeclass version of ValidCtxInd *)
+Class ValidCtx ctx : Prop :=
+  validCtx : ValidCtxInd ctx.
+
+(* Instances for building ValidCtx proofs *)
+Instance ValidCtx_Nil : ValidCtx CtxNil := ValidCtxNil.
+Instance ValidCtx_Cons A `{OType A} ctx (vc:ValidCtx ctx) :
+  ValidCtx (CtxCons A ctx) := ValidCtxCons A ctx vc.
 
 (* An element of a context is a nested tuple of elements of its types *)
 Fixpoint CtxElem (ctx:Ctx) : Type :=
@@ -94,73 +54,245 @@ Proof.
   - apply OTpair_R; assumption.
 Defined.
 
-(* Inductive type stating that every type in a Ctx is a valid OType *)
-Inductive ValidCtxInd : Ctx -> Prop :=
-| ValidCtxNil : ValidCtxInd CtxNil
-| ValidCtxCons A `{OType A} ctx : ValidCtxInd ctx -> ValidCtxInd (CtxCons A ctx)
-.
-
-(* Typeclass version of ValidCtxInd *)
-Class ValidCtx ctx : Prop :=
-  validCtx : ValidCtxInd ctx.
-
-(* Instances for building ValidCtx proofs *)
-Instance ValidCtx_Nil : ValidCtx CtxNil := ValidCtxNil.
-Instance ValidCtx_Cons A `{OType A} ctx (vc:ValidCtx ctx) :
-  ValidCtx (CtxCons A ctx) := ValidCtxCons A ctx vc.
-
 (* OType instance of CtxElem of a valid context *)
 Instance OType_CtxElem ctx (valid:ValidCtx ctx) : OType (CtxElem ctx).
 Proof.
   induction valid; typeclasses eauto.
 Qed.
 
-(* Proofs that a type is the nth element of a context *)
-Fixpoint HasTypeVar (v:nat) (ctx:Ctx) (B:Type) {RB:OTRelation B} : Prop :=
-  match v with
-  | 0 =>
-    match ctx with
-    | CtxNil => False
-    | @CtxCons A RA _ => eqOType A B
-    end
-  | S v' =>
-    match ctx with
-    | CtxNil => False
-    | CtxCons _ ctx' => HasTypeVar v' ctx' B
+(* Look up the nth type in a Ctx, returning the unit type as a default *)
+Fixpoint nthCtx n ctx {struct ctx} : Type :=
+  match ctx with
+  | CtxNil => unit
+  | CtxCons A ctx' =>
+    match n with
+    | 0 => A
+    | S n' => nthCtx n' ctx'
     end
   end.
 
-(* Typing proofs for ordered expressions *)
-Fixpoint HasType (e:OExpr) (ctx:Ctx) (B:Type) {RB:OTRelation B} : Prop :=
-  match e with
-  | OVar v => HasTypeVar v ctx B
-  | @OEmbed A RA a => eqOType A B /\ OType A
-  | OApp A B' f arg =>
-    eqOType B' B /\ (HasType f ctx (A -o> B') /\ HasType arg ctx A)
-  | OLam A B' body =>
-    eqOType (A -o> B') B /\ (ValidCtx ctx /\ HasType body (CtxCons A ctx) B')
-  end.
+(* The OTRelation for the nth type in a context *)
+Instance OTRelation_nthCtx n ctx : OTRelation (nthCtx n ctx).
+Proof.
+  revert n; induction ctx; intros; simpl; try typeclasses eauto.
+  destruct n; simpl; typeclasses eauto.
+Defined.
 
-(* Lemma: each HasTypeVar proof is unique *)
-(*
-Lemma HasTypeVar_unique v ctx B {RB:OTRelation B} (ht1 ht2: HasTypeVar v ctx B)
-  : ht1 = ht2.
-  revert ctx ht1 ht2; induction v; destruct ctx; simpl; intros;
-    try apply proof_irrelevance; try apply IHv; try destruct ht1.
+(* For valid contexts, the nth element is a valid OType *)
+Instance OType_nthCtx n ctx `{valid:ValidCtx ctx} : OType (nthCtx n ctx).
+Proof.
+  revert n valid; induction ctx; intros; simpl; try typeclasses eauto.
+  destruct (ValidCtxInd_inversion _ _ valid).
+  destruct n; try assumption. apply IHctx; apply H1.
 Qed.
+
+(* Get the head type of a context, defaulting to unit *)
+Definition ctxHead ctx : Type :=
+  match ctx with
+  | CtxNil => unit
+  | CtxCons A _ => A
+  end.
+
+Instance OTRelation_ctxHead ctx : OTRelation (ctxHead ctx) :=
+  match ctx with
+  | CtxNil => _
+  | CtxCons _ _ => _
+  end.
+
+Instance OType_ctxHead ctx `{valid:ValidCtx ctx} : OType (ctxHead ctx).
+Proof.
+  destruct ctx.
+  - typeclasses eauto.
+  - exact (proj1 (ValidCtxInd_inversion _ ctx valid)).
+Qed.
+
+(* Get the tail of a context, defaulting to the empty context *)
+Definition ctxTail ctx :=
+  match ctx with
+  | CtxNil => CtxNil
+  | CtxCons _ ctx' => ctx'
+  end.
+
+Instance ValidCtx_ctxTail ctx `{valid:ValidCtx ctx} : ValidCtx (ctxTail ctx).
+Proof.
+  destruct ctx.
+  - typeclasses eauto.
+  - exact (proj2 (ValidCtxInd_inversion _ ctx valid)).
+Qed.
+
+(* Non-nil contexts equal cons of their heads and tails *)
+Lemma ctx_eq_head_tail ctx :
+  ctx <> CtxNil -> ctx = CtxCons (ctxHead ctx) (ctxTail ctx).
+  destruct ctx; intro e.
+  elimtype False; apply e; reflexivity.
+  reflexivity.
+Qed.
+
+(* Appending contexts *)
+Fixpoint appendCtx ctx1 ctx2 : Ctx :=
+  match ctx1 with
+  | CtxNil => ctx2
+  | CtxCons A ctx1' =>
+    CtxCons A (appendCtx ctx1' ctx2)
+  end.
+
+(* Context length *)
+Fixpoint ctxLen ctx :=
+  match ctx with
+  | CtxNil => 0
+  | CtxCons A ctx' => S (ctxLen ctx')
+  end.
+
+
+(***
+ *** Semantic Types
+ ***)
+
+(* A "semantics type", which is a context plus an ordered type *)
+Record SemType : Type :=
+  { semCtx : Ctx;
+    semType : Type;
+    sem_OTRelation :> OTRelation semType }.
+
+(* For some reason, Coq doesn't build sem_OTRelation as an instance... *)
+Instance OTRelation_SemType semTp : OTRelation (semType semTp) :=
+  sem_OTRelation semTp.
+
+(* Typeclass capturing that a SemType is valid: semType is an OType *)
+Class ValidSemType semTp : Prop := otypeSemType :> OType (semType semTp).
+
+(* Convert a SemType to an actual type (FIXME: should this be a coercion?) *)
+Definition oSemantics (semTp:SemType) : Type :=
+  CtxElem (semCtx semTp) -o> semType semTp.
+
+(* Cast a semantic value to an equal semantic type *)
+Definition castSemantics {semTp1 semTp2} (e:semTp1=semTp2)
+           (sem:oSemantics semTp1) : oSemantics semTp2 :=
+  rew e in sem.
+
+(* castSemantics is Proper *)
+Instance Proper_castSemantics semTp1 semTp2 (e:semTp1=semTp2) :
+  Proper (ot_R ==> ot_R) (castSemantics e).
+Proof.
+  generalize e. rewrite e. intros e2 sem1 sem2 Rsem.
+  rewrite (UIP_refl _ _ e2). apply Rsem.
+Qed.
+
+Lemma double_cast {A} {x y z:A} {F:A -> Type} (e1:x=y) (e2:y=z) (e3:x=z) obj :
+  rew [F] e2 in (rew [F] e1 in obj) = rew [F] e3 in obj.
+  revert e2 e3 obj. generalize e1. rewrite e1. intros. rewrite (UIP_refl _ _ e0).
+  simpl. rewrite (UIP _ _ _ e2 e3). reflexivity.
+Qed.
+
+(* A cast of a cast is a cast *)
+Definition double_castSemantics semTp1 semTp2 semTp3 (e1:semTp1=semTp2)
+           (e2:semTp2=semTp3) e3 sem :
+  castSemantics e2 (castSemantics e1 sem) = castSemantics e3 sem :=
+  double_cast _ _ _ _.
+
+
+FIXME HERE NOW: we need to prove that castSemantics commutes with exprSemantics
+for the OApp and OLam constructors, which is going to be gross...
+
+
+(* castSemantics commutes with pfun_apply *)
+Lemma castSemantics_pfun_apply_commute semTp1 semTp2 (e:semTp1=semTp2)
+      (fsem: oSemantics {| semCtx := semCtx semTp1 |})
+
+
+(***
+ *** Ordered Expressions
+ ***)
+
+(* Ordered expressions to represent proper functions *)
+Inductive OExpr : Type :=
+| OVar (ctx:Ctx) (n:nat)
+| OEmbed (ctx:Ctx) {A} {RA:OTRelation A} (a:A)
+| OApp (B:Type) {RB:OTRelation B} (e1 e2 : OExpr)
+| OLam (e: OExpr)
+.
+
+(* We can always look up the correct context and ordered type of an OExpr *)
+Fixpoint OExpr_SemType (e:OExpr) : SemType :=
+  match e with
+  | OVar ctx n => Build_SemType ctx (nthCtx n ctx) _
+  | @OEmbed ctx A _ _ => Build_SemType ctx A _
+  | OApp B _ arg => Build_SemType (semCtx (OExpr_SemType arg)) B _
+  | OLam f =>
+    Build_SemType (ctxTail (semCtx (OExpr_SemType f)))
+                  (ctxHead (semCtx (OExpr_SemType f)) -o> semType (OExpr_SemType f))
+                  _
+  end.
+
+Definition OExpr_ctx e := semCtx (OExpr_SemType e).
+Definition OExpr_type e := semType (OExpr_SemType e).
+Instance OTRelation_OExpr_type e : OTRelation (OExpr_type e) := _.
+
+
+(***
+ *** Substitution and Weakening for Ordered Expressions
+ ***)
+
+(* Weakening / lifting of ordered expression variables: insert w_ctx into the
+context of a variable at point n *)
+Fixpoint weakenOVar n w_ctx (v:nat) {struct n} : nat :=
+  match n with
+  | 0 => v + ctxLen w_ctx
+  | S n' =>
+    match v with
+    | 0 => 0
+    | S v' => weakenOVar n' w_ctx v'
+    end
+  end.
+
+(* Weakening a context by inserting another at point n *)
+Fixpoint weakenCtx n w_ctx ctx : Ctx :=
+  match n with
+  | 0 => appendCtx w_ctx ctx
+  | S n' =>
+    match ctx with
+    | CtxNil => CtxCons unit (weakenCtx n' w_ctx CtxNil)
+    | CtxCons A ctx' => CtxCons A (weakenCtx n' w_ctx ctx')
+    end
+  end.
+
+(* Weakening / lifting of ordered expressions *)
+Fixpoint weakenOExpr n w_ctx (e:OExpr) : OExpr :=
+  match e with
+  | OVar ctx v => OVar (weakenCtx n w_ctx ctx) (weakenOVar n w_ctx v)
+  | OEmbed ctx a => OEmbed (weakenCtx n w_ctx ctx) a
+  | OApp B f arg =>
+    OApp B (weakenOExpr n w_ctx f) (weakenOExpr n w_ctx arg)
+  | OLam f => OLam (weakenOExpr (S n) w_ctx f)
+  end.
+
+(* Substitution for ordered expression variables *)
+(* FIXME HERE: write this!
+Fixpoint substOVar n w_ctx (s:OExpr) v : OExpr :=
+  match n with
+  | 0 =>
+    match v with
+    | 0 => weakenOExpr 0 w_ctx s
+    | S v' => OVar v'
+    end
+  | S n' =>
+    match v with
+    | 0 => OVar lifting
+    | S v' =>
+      substOVar n' (S lifting) s v
+    end
+  end.
 *)
 
-(* Lemma: each HasType proof is unique *)
+(* Substitution for ordered expressions *)
 (*
-Lemma HasType_unique ctx B {RB:OTRelation B} e (ht1 ht2: HasType e ctx B)
-  : ht1 = ht2.
-  revert ctx B RB ht1 ht2; induction e; simpl; intros.
-  { apply HasTypeVar_unique. }
-  { apply proof_irrelevance. }
-  { destruct ht1; destruct ht2; f_equal; apply proof_irrelevance. }
-      repeat f_equal; first [ apply UIP | apply IHe1 | apply IHe2 ]. }
-  { destruct ht1; destruct ht2. f_equal; [ apply UIP | apply IHe ]. }
-Qed.
+Fixpoint substOExpr n (s:OExpr) (e:OExpr) : OExpr :=
+  match e with
+  | OVar v => substOVar n CtxNil s v
+  | OEmbed a => OEmbed a
+  | OApp A B f arg => OApp A B (substOExpr n s f) (substOExpr n s arg)
+  | OLam A B body => OLam A B (substOExpr (S n) s body)
+  end.
  *)
 
 
@@ -168,104 +300,176 @@ Qed.
  *** The Semantics of Ordered Expressions
  ***)
 
-(* The semantics of a well-typed variable *)
-Program Fixpoint varSemantics v ctx B {RB:OTRelation B} :
-  HasTypeVar v ctx B -> CtxElem ctx -o> B :=
-  match v return HasTypeVar v ctx B -> CtxElem ctx -o> B with
-  | 0 =>
-    match ctx return HasTypeVar 0 ctx B -> CtxElem ctx -o> B with
-    | CtxNil => fun ht => match ht with end
-    | @CtxCons A RA ctx' =>
-      fun ht =>
-        rew [fun p =>
-               @Pfun (CtxElem ctx' * A) (projT1 p) (OTpair_R _ A _ RA) (projT2 p)]
-            ht in (snd_pfun (B:=projT1 (existT OTRelation A RA)))
-    end
-  | S v' =>
-    match ctx return HasTypeVar (S v') ctx B ->
-                     @Pfun (CtxElem ctx) B (OTRelation_CtxElem ctx) _ with
-    | CtxNil => fun ht => match ht with end
-    | CtxCons A ctx' =>
-      fun ht =>
-        compose_pfun fst_pfun (varSemantics v' ctx' B ht)
+Definition oexprSemantics e := oSemantics (OExpr_SemType e).
+
+
+(* Since expressions contain their types and contexts, the only requirement for
+typing ordered expressions is that different parts of the expression have types
+that agree with each other, and that the contexts are always valid *)
+Fixpoint WellTypedP (e:OExpr) : Prop :=
+  match e with
+  | OVar ctx n => ValidCtx ctx
+  | @OEmbed ctx A _ a => ValidCtx ctx /\ OType A
+  | OApp B f arg =>
+    (OExpr_SemType f =
+     {| semCtx := OExpr_ctx arg; semType := OExpr_type arg -o> B;
+        sem_OTRelation := _ |} /\ OType B)
+    /\ (WellTypedP f /\ WellTypedP arg)
+  | OLam f =>
+    OExpr_SemType f =
+    {| semCtx := CtxCons (ctxHead (OExpr_ctx f)) (ctxTail (OExpr_ctx f));
+       semType := OExpr_type f; sem_OTRelation := _ |}
+    /\ WellTypedP f
+  end.
+
+(* Type class for well-typedness *)
+Class WellTyped e : Prop := wellTyped : WellTypedP e.
+
+(* Any WellTyped expression has a ValidCtx *)
+Instance ValidCtx_OExpr_ctx e (wt:WellTyped e) : ValidCtx (OExpr_ctx e).
+Proof.
+  revert wt; induction e; simpl; intro wt.
+  - assumption.
+  - exact (proj1 wt).
+  - apply IHe2. apply (proj2 (proj2 wt)).
+  - apply ValidCtx_ctxTail. apply IHe. apply (proj2 wt).
+Qed.
+
+(* Any WellTyped expression has a valid type *)
+Instance OType_OExpr_type e (wt:WellTyped e) : OType (OExpr_type e).
+Proof.
+  revert wt; induction e; simpl; intro wt.
+  - typeclasses eauto.
+  - destruct wt; assumption.
+  - destruct wt as [wt1 wt2]; destruct wt1; assumption.
+  - unfold OExpr_type. simpl. destruct wt. typeclasses eauto.
+Qed.
+
+(* The semantics of a variable *)
+Fixpoint varSemantics ctx v {struct ctx} :
+  oSemantics (Build_SemType ctx (nthCtx v ctx) _) :=
+  match ctx return oSemantics (Build_SemType ctx (nthCtx v ctx) _) with
+  | CtxNil => const_pfun tt
+  | CtxCons A ctx' =>
+    match v return
+          oSemantics (Build_SemType (CtxCons A ctx') (nthCtx v (CtxCons A ctx')) _)
+    with
+    | 0 => snd_pfun
+    | S v' => compose_pfun fst_pfun (varSemantics ctx' v')
     end
   end.
 
-(* Helper to cast a proper function using an equality on ordered types *)
-Definition castSemantics {ctx A B} `{OTRelation A} `{OTRelation B}
-           (e:eqOType A B) (sem: CtxElem ctx -o> A) : CtxElem ctx -o> B :=
-  rew [fun p => @Pfun (CtxElem ctx) (projT1 p) _ (projT2 p)] e in
-    (sem : CtxElem ctx -o> (projT1 (existT OTRelation A _))).
 
 (* The semantics of a well-typed expression *)
-Fixpoint exprSemantics e ctx B {RB:OTRelation B} :
-  HasType e ctx B -> CtxElem ctx -o> B :=
-  match e return HasType e ctx B -> CtxElem ctx -o> B with
-  | OVar v => varSemantics v ctx B
-  | OEmbed a =>
-    fun ht => castSemantics (proj1 ht) (const_pfun (H0:=proj2 ht) a)
-  | OApp A B' f arg =>
-    fun ht =>
-      castSemantics
-        (proj1 ht)
-        (pfun_apply
-           (exprSemantics f ctx (A -o> B') (proj1 (proj2 ht)))
-           (exprSemantics arg ctx A (proj2 (proj2 ht))))
-  | OLam A B' body =>
-    fun ht =>
-      castSemantics
-        (proj1 ht)
-        (pfun_curry (H:=OType_CtxElem ctx (proj1 (proj2 ht)))
-                   (exprSemantics body (CtxCons A ctx) B' (proj2 (proj2 ht)))
-         : CtxElem ctx -o> (projT1 (existT OTRelation (A -o> B') _)))
+Program Fixpoint exprSemantics e :
+  forall `{WellTyped e}, oexprSemantics e :=
+  match e return WellTyped e -> oexprSemantics e with
+  | OVar ctx v =>
+    fun wt => varSemantics ctx v
+  | OEmbed ctx a =>
+    fun wt => const_pfun (H0:=proj2 wt) a
+  | OApp B f arg =>
+    fun wt =>
+      pfun_apply
+        (castSemantics (proj1 (proj1 wt)) (@exprSemantics f (proj1 (proj2 wt))))
+        (@exprSemantics arg (proj2 (proj2 wt)))
+  | OLam f =>
+    fun wt =>
+      pfun_curry
+        (H:= _ )
+        (castSemantics (proj1 wt) (@exprSemantics f (proj2 wt)))
   end.
+Next Obligation.
+  eauto with typeclass_instances.
+Defined.
+
+Instance OTRelation_expr_oSemantics e : OTRelation (oexprSemantics e) := _.
+Instance OType_expr_oSemantics e (wt:WellTyped e) :
+  OType (oexprSemantics e) := _.
+
+(* castSemantics commutes with the semantics of applications *)
+Lemma castSemantics_commute_OApp B B' {RB:OTRelation B} {RB':OTRelation B} e1 e2
 
 
 (***
  *** Relating Ordered Expressions
  ***)
 
-(* The preorder on ordered expressions *)
-Definition oexpr_R ctx B `{OTRelation B} : relation OExpr :=
-  fun e1 e2 =>
-    (HasType e1 ctx B <-> HasType e2 ctx B) /\
-    (forall ht1 ht2 `{ValidCtx ctx},
-        ot_R (exprSemantics e1 ctx B ht1) (exprSemantics e2 ctx B ht2)).
+Record oexpr_R (e1 e2:OExpr) : Prop :=
+  { oexpr_R_wt : WellTyped e1 <-> WellTyped e2;
+    oexpr_R_eq_tp : OExpr_SemType e1 = OExpr_SemType e2;
+    oexpr_R_sem :
+      forall wt1 wt2,
+        castSemantics oexpr_R_eq_tp (@exprSemantics e1 wt1) <o=
+        @exprSemantics e2 wt2 }.
 
 (* The equivalence relation on ordered expressions *)
-Definition oexpr_eq ctx B `{OTRelation B} : relation OExpr :=
-  fun e1 e2 => oexpr_R ctx B e1 e2 /\ oexpr_R ctx B e2 e1.
+Definition oexpr_eq : relation OExpr :=
+  fun e1 e2 => oexpr_R e1 e2 /\ oexpr_R e2 e1.
 
 (* oexpr_R is reflexive *)
-Instance Reflexive_oexpr_R ctx B `{OType B} : Reflexive (oexpr_R ctx B).
+Instance Reflexive_oexpr_R : Reflexive oexpr_R.
 Proof.
-  intro e; split; intros.
+  intro e; split.
   - reflexivity.
-  - rewrite (proof_irrelevance _ ht1 ht2); apply pfun_Proper; assumption.
+  - intros; apply mk_otRdep. rewrite (proof_irrelevance _ wt1 wt2). reflexivity.
 Qed.
 
 (* oexpr_R is transitive *)
-Instance Transitive_oexpr_R ctx B `{OType B} : Transitive (oexpr_R ctx B).
+Instance Transitive_oexpr_R : Transitive oexpr_R.
 Proof.
-  intros e1 e2 e3 r12 r23; destruct r12; destruct r23; split.
-  { transitivity (HasType e2 ctx B); [ apply H0 | apply H2 ]. }
-  { intros ht1 ht3 valid.
-    assert (HasType e2 ctx B) as ht2; [ apply H0; assumption | ].
-    transitivity (exprSemantics e2 ctx B ht2).
-    - apply H1; assumption.
-    - apply H3; assumption. }
+  intros e1 e2 e3 [ wt12 r12 ]. destruct 
+  split.
+  { transitivity (WellTyped e2); assumption. }
+  { intros wt1 wt3. rewrite <- r23. rewrite <- r12.
+    rewrite (double_castSemantics _ _ _ _ _ (eq_trans eq12 eq23)).
+    reflexivity. }
+  Unshelve.
+  apply wt23. assumption.
 Qed.
 
 (* oexpr_R is thus a PreOrder *)
-Instance PreOrder_oexpr_R ctx B `{OType B} : PreOrder (oexpr_R ctx B) :=
+Instance PreOrder_oexpr_R : PreOrder oexpr_R :=
   Build_PreOrder _ _ _.
 
 (* oexpr_eq is thus an Equivalence *)
-Instance Equivalence_oexpr_eq ctx B `{OType B} : Equivalence (oexpr_eq ctx B).
+Instance Equivalence_oexpr_eq : Equivalence oexpr_eq.
 Proof.
   constructor; intro; intros.
   { split; reflexivity. }
-  { destruct H0; split; assumption. }
-  { destruct H0; destruct H1; split; transitivity y; assumption. }
+  { destruct H; split; assumption. }
+  { destruct H; destruct H0; split; transitivity y; assumption. }
 Qed.
 
+
+(***
+ *** Rewriting Relative to oexpr_R and oexpr_eq
+ ***)
+
+Instance Proper_OEmbed_R ctx A {RA:OTRelation A} :
+  Proper (ot_R ==> oexpr_R) (@OEmbed ctx A _).
+Proof.
+  intros a1 a2 Ra. split; [ | exists eq_refl ].
+  { reflexivity. }
+  { unfold castSemantics; simpl; intros. rewrite (proof_irrelevance _ wt1 wt2).
+    destruct wt1. rewrite Ra. reflexivity. }
+Qed.
+
+Instance Proper_OEmbed_eq ctx A {RA:OTRelation A} :
+  Proper (ot_equiv ==> oexpr_eq) (@OEmbed ctx A _).
+Proof.
+  intros a1 a2 eqA; destruct eqA; split; apply Proper_OEmbed_R; assumption.
+Qed.
+
+Instance Proper_OApp_R (B:Type) {RB:OTRelation B} :
+  Proper (oexpr_R ==> oexpr_R ==> oexpr_R) (OApp B).
+Proof.
+  intros f1 f2 [ wt_f [ eqf rf ] ] arg1 arg2 [ wt_a [ eqa ra ] ].
+  split; [ | eexists ]. Unshelve.
+  { simpl. rewrite eqf. unfold OExpr_ctx, OExpr_type, OTRelation_OExpr_type.
+    rewrite wt_f. rewrite wt_a. rewrite eqa. reflexivity. }
+  { simpl; intros.
+
+ intro wt1; generalize wt1. 
+
+ intros.
